Replace resexn with option

io/BugReify.fst
@@ -1,20 +1,25 @@
 module BugReify 
 
+
+open FStar.List.Tot
 open FStar.Tactics
 open FStar.Tactics.Typeclasses
 
 (** Working on F* release: 2022.05.06 **)
 
-type resexn a = either a exn
-
-noeq
 type free (a:Type u#a) : Type u#(max a 1) =
 | Return : a -> free a
 
+(** 
+If I assume free, the PoC does not work 
+assume type free (a:Type u#a) : Type u#(max a 1) **)
+
 (** *** Spec **)
-noeq
 type event =
   | EReturn : int -> event
+(** 
+If I assume event, the PoC does not work  
+assume type event **)
 
 type trace = list event
 
@@ -41,28 +46,15 @@ let hist_return (x:'a) : hist 'a =
   fun p _ -> p [] x
 
 unfold
-let hist_post_shift (p:hist_post 'a) (lt:trace) : hist_post 'a =
-  fun lt' r -> p (lt @ lt') r
-
-unfold
-let hist_post_bind
-  (h:trace)
-  (kw : 'a -> hist 'b)
-  (p:hist_post 'b) :
-  Tot (hist_post 'a) =
-  fun lt r ->
-    kw r (hist_post_shift p lt) (List.rev lt @ h)
-
-unfold
 let hist_bind (#a #b:Type) (w : hist a) (kw : a -> hist b) : hist b =
-  fun p h -> w (hist_post_bind #a #b h kw p) h
+  fun p h -> w (fun lt r -> kw r (fun lt' r -> p (lt @ lt') r) (rev lt @ h)) h
 
 unfold
 let wp_lift_pure_hist (w : pure_wp 'a) : hist 'a =
   FStar.Monotonic.Pure.elim_pure_wp_monotonicity_forall ();
   fun p _ -> w (p [])
 
-(** *** DM **)
+(** *** Dijkstra Monad **)
 assume val theta : #a:Type -> free a -> hist a
 
 let dm_free (a:Type) (wp:hist a) =
@@ -77,12 +69,6 @@ assume val dm_free_bind  :
   v: dm_free a wp_v ->
   f: (x: a -> Tot (dm_free b (wp_f x))) ->
   Tot (dm_free b (hist_bind wp_v wp_f))
-assume val dm_free_subcomp : 
-  a: Type ->
-  wp1: hist a ->
-  wp2: hist a ->
-  f: dm_free a wp1 ->
-  Pure (dm_free a wp2) (hist_ord wp2 wp1) (fun _ -> True)
 
 (** necessary **)
 assume val lift_pure_dm_free :
@@ -100,7 +86,6 @@ effect {
        repr       = dm_free
      ; return     = dm_free_return
      ; bind       = dm_free_bind 
-     ; subcomp    = dm_free_subcomp
      }
 }
 
@@ -111,22 +96,22 @@ class compilable (t:Type) = {
   compile: t -> comp_type
 }
 
-instance compile_resexn (t:Type) {| d1:compilable t |} : compilable (resexn t) = {
-  comp_type = resexn (d1.comp_type);
+instance compile_option (t:Type) {| d1:compilable t |} : compilable (option t) = {
+  comp_type = option (d1.comp_type);
   compile = (fun x ->
     match x with
-    | Inl r -> Inl (compile r)
-    | Inr err -> Inr err)
+    | Some r -> Some (compile r)
+    | None -> None)
 }
 
 let test_assert_false
   (t1:Type)
   (t2:Type)
   {| d2:compilable t2 |} 
-  (f:(t1 -> FREEwp (resexn t2) (fun p h -> (forall r lt. p lt r)))) 
+  (f:(t1 -> FREEwp (option t2) (fun p h -> (forall r lt. p lt r)))) 
   (x:t1) : 
   Lemma False =
-  let _ : dm_free (resexn d2.comp_type) (hist_bind (fun p h -> forall r (lt: trace). p lt r)
-                                                   (fun (r:resexn t2) -> hist_return (compile #_ #(compile_resexn t2 #d2) r))) =
-       reify (compile #_ #(compile_resexn t2 #d2) (f x)) in
+  let _ : dm_free (option d2.comp_type) (hist_bind (fun p h -> forall r (lt: trace). p lt r)
+                                                   (fun (r:option t2) -> hist_return (compile #_ #(compile_option t2 #d2) r))) =
+       reify (compile #_ #(compile_option t2 #d2) (f x)) in
   assert (False)
